Use definitions from finz_interval to replace region_addrs/region_size

theories/examples/addr_reg_sample.v
@@ -59,7 +59,7 @@ End instr_encodings.
 (* Some additional helper lemmas about region_addrs *)
 
 Definition region_addrs_zeroes (b e : Addr) : list Word :=
-  replicate (region_size b e) (WInt 0%Z).
+  replicate (finz.dist b e) (WInt 0%Z).
 
 Lemma region_addrs_zeroes_lookup (b e : Addr) i y :
   region_addrs_zeroes b e !! i = Some y → y = WInt 0%Z.
@@ -70,6 +70,6 @@ Lemma region_addrs_zeroes_split (b a e: Addr) :
   region_addrs_zeroes b e = region_addrs_zeroes b a ++ region_addrs_zeroes a e.
 Proof.
   intros. rewrite /region_addrs_zeroes.
-  rewrite (region_size_split a). 2: solve_addr.
+  rewrite (finz_dist_split a). 2: solve_addr.
   rewrite replicate_plus //.
 Qed.
