theories/examples/mkregion_helpers.v
@@ -8,19 +8,19 @@ From cap_machine Require Import stdpp_extra iris_extra cap_lang
 From cap_machine.examples Require Import disjoint_regions_tactics.
 
 Definition mkregion (r_start r_end: Addr) (contents: list Word): gmap Addr Word :=
-  list_to_map (zip (region_addrs r_start r_end) contents).
+  list_to_map (zip (finz.seq_between r_start r_end) contents).
 
-Lemma zip_region_addrs_lookup {A} (b e a : Addr) (l : list A) x :
+Lemma zip_seq_between_lookup {A} (b e a : Addr) (l : list A) x :
   (b + length l = Some e)%a →
-  (a, x) ∈ zip (region_addrs b e) l ↔ ∃ (i:nat), a = (b ^+ i)%a ∧ l !! i = Some x.
+  (a, x) ∈ zip (finz.seq_between b e) l ↔ ∃ (i:nat), a = (b ^+ i)%a ∧ l !! i = Some x.
 Proof.
   revert b e a x. induction l as [| x l].
   { intros * Hl. cbn.
     rewrite (_: b = e). 2: solve_addr.
-    rewrite region_addrs_empty //. 2: solve_addr. cbn.
+    rewrite finz_seq_between_empty //. 2: solve_addr. cbn.
     split. by inversion 1. intros [? [? ?] ]. congruence. }
   { intros * Hl. cbn in *.
-    rewrite region_addrs_cons. 2: solve_addr. cbn.
+    rewrite finz_seq_between_cons. 2: solve_addr. cbn.
     split.
     { intros [HH|HH]%elem_of_cons.
       { simplify_eq. exists 0. split. solve_addr. constructor. }
@@ -47,8 +47,8 @@ Lemma mkregion_app l1 l2 b e :
   mkregion b (b ^+ length l1)%a l1 ∪ mkregion (b ^+ length l1)%a e l2.
 Proof.
   rewrite /mkregion. rewrite app_length. intros HH.
-  rewrite (region_addrs_split _ (b ^+ length l1)%a). 2: split; solve_addr.
-  rewrite zip_app. 2: rewrite region_addrs_length /region_size; solve_addr.
+  rewrite (finz_seq_between_split _ (b ^+ length l1)%a). 2: split; solve_addr.
+  rewrite zip_app. 2: rewrite finz_seq_between_length /finz.dist; solve_addr.
   rewrite list_to_map_app //.
 Qed.
 
@@ -57,15 +57,15 @@ Lemma mkregion_lookup (b e a : Addr) l x :
   mkregion b e l !! a = Some x ↔ ∃ (i:nat), a = (b ^+ i)%a ∧ l !! i = Some x.
 Proof.
   intros Hl. rewrite /mkregion.
-  rewrite -elem_of_list_to_map. apply zip_region_addrs_lookup; auto.
-  rewrite fst_zip. apply region_addrs_NoDup.
-  rewrite region_addrs_length /region_size. solve_addr.
+  rewrite -elem_of_list_to_map. apply zip_seq_between_lookup; auto.
+  rewrite fst_zip. apply finz_seq_between_NoDup.
+  rewrite finz_seq_between_length /finz.dist. solve_addr.
 Qed.
 
 Lemma dom_mkregion_incl a e l:
-  dom (gset Addr) (mkregion a e l) ⊆ list_to_set (region_addrs a e).
+  dom (gset Addr) (mkregion a e l) ⊆ list_to_set (finz.seq_between a e).
 Proof.
-  rewrite /mkregion. generalize (region_addrs a e). induction l.
+  rewrite /mkregion. generalize (finz.seq_between a e). induction l.
   { intros. rewrite zip_with_nil_r /=. rewrite dom_empty_L. apply empty_subseteq. }
   { intros ll. destruct ll as [| x ll].
     - cbn. rewrite dom_empty_L. done.
@@ -75,12 +75,12 @@ Qed.
 
 Lemma dom_mkregion_incl_rev a e l:
   (a + length l = Some e)%a →
-  list_to_set (region_addrs a e) ⊆ dom (gset Addr) (mkregion a e l).
+  list_to_set (finz.seq_between a e) ⊆ dom (gset Addr) (mkregion a e l).
 Proof.
   rewrite /mkregion. intros Hl.
-  assert (length (region_addrs a e) = length l) as Hl'.
-  { rewrite region_addrs_length /region_size. solve_addr. }
-  clear Hl. revert Hl'. generalize (region_addrs a e). induction l.
+  assert (length (finz.seq_between a e) = length l) as Hl'.
+  { rewrite finz_seq_between_length /finz.dist. solve_addr. }
+  clear Hl. revert Hl'. generalize (finz.seq_between a e). induction l.
   { intros. rewrite zip_with_nil_r /=. rewrite dom_empty_L.
     destruct l; [| inversion Hl']. cbn. apply empty_subseteq. }
   { intros ll Hll. destruct ll as [| x ll]; [by inversion Hll|].
@@ -91,7 +91,7 @@ Qed.
 
 Lemma dom_mkregion_eq a e l:
   (a + length l = Some e)%a →
-  dom (gset Addr) (mkregion a e l) = list_to_set (region_addrs a e).
+  dom (gset Addr) (mkregion a e l) = list_to_set (finz.seq_between a e).
 Proof.
   intros Hlen. apply (anti_symm _).
   - apply dom_mkregion_incl.
@@ -100,7 +100,7 @@ Qed.
 
 Lemma in_dom_mkregion a e l k:
   k ∈ dom (gset Addr) (mkregion a e l) →
-  k ∈ region_addrs a e.
+  k ∈ finz.seq_between a e.
 Proof.
   intros H.
   pose proof (dom_mkregion_incl a e l) as HH.
@@ -111,7 +111,7 @@ Qed.
 
 Lemma in_dom_mkregion' a e l k:
   (a + length l = Some e)%a →
-  k ∈ region_addrs a e →
+  k ∈ finz.seq_between a e →
   k ∈ dom (gset Addr) (mkregion a e l).
 Proof.
   intros. rewrite dom_mkregion_eq // elem_of_list_to_set //.
@@ -135,22 +135,22 @@ Ltac disjoint_map_to_list :=
 
 Lemma mkregion_sepM_to_sepL2 `{Σ: gFunctors} (a e: Addr) l (φ: Addr → Word → iProp Σ) :
   (a + length l)%a = Some e →
-  ⊢ ([∗ map] k↦v ∈ mkregion a e l, φ k v) -∗ ([∗ list] k;v ∈ (region_addrs a e); l, φ k v).
+  ⊢ ([∗ map] k↦v ∈ mkregion a e l, φ k v) -∗ ([∗ list] k;v ∈ (finz.seq_between a e); l, φ k v).
 Proof.
   rewrite /mkregion. revert a e. induction l as [| x l].
   { cbn. intros. rewrite zip_with_nil_r /=. assert (a = e) as -> by solve_addr.
-    rewrite /region_addrs region_size_0. 2: solve_addr. cbn. eauto. }
-  { cbn. intros a e Hlen. rewrite region_addrs_cons. 2: solve_addr.
+    rewrite /finz.seq_between finz_dist_0. 2: solve_addr. cbn. eauto. }
+  { cbn. intros a e Hlen. rewrite finz_seq_between_cons. 2: solve_addr.
     cbn. iIntros "H". iDestruct (big_sepM_insert with "H") as "[? H]".
     { rewrite -not_elem_of_list_to_map /=.
-      intros [ [? ?] [-> [? ?]%elem_of_zip_l%elem_of_region_addrs] ]%elem_of_list_fmap.
+      intros [ [? ?] [-> [? ?]%elem_of_zip_l%elem_of_finz_seq_between] ]%elem_of_list_fmap.
       solve_addr. }
     iFrame. iApply (IHl with "H"). solve_addr. }
 Qed.
 
 Lemma mkregion_prepare `{memG Σ} (a e: Addr) l :
   (a + length l)%a = Some e →
-  ⊢ ([∗ map] k↦v ∈ mkregion a e l, k ↦ₐ v) ==∗ ([∗ list] k;v ∈ (region_addrs a e); l, k ↦ₐ v).
+  ⊢ ([∗ map] k↦v ∈ mkregion a e l, k ↦ₐ v) ==∗ ([∗ list] k;v ∈ (finz.seq_between a e); l, k ↦ₐ v).
 Proof.
   iIntros (?) "H". iDestruct (mkregion_sepM_to_sepL2 with "H") as "H"; auto.
 Qed.
